Rewrite.

theories/language/itype.v
@@ -9,96 +9,96 @@ Class iType (PROP : bi) (τ : val → PROP) := {
   #[global] itype_persistent v :: Persistent (τ v) ;
 }.
 
-Section basic_types.
+Section basic.
   Context {PROP : bi}.
 
   Implicit Types v : val.
 
-  Definition bool_type v : PROP :=
-    ∃ b, ⌜v = ValLiteral (LiteralBool b)⌝.
-  #[global] Instance bool_type_itype :
-    iType _ bool_type.
-  Proof.
-    split. apply _.
-  Qed.
-
-  Definition unit_type v : PROP :=
+  Definition itype_unit v : PROP :=
     ⌜v = ValUnit⌝.
-  #[global] Instance unit_type_itype :
-    iType _ unit_type.
+  #[global] Instance itype_unit_itype :
+    iType _ itype_unit.
   Proof.
     split. apply _.
   Qed.
 
-  Definition int_type v : PROP :=
+  Definition itype_bool v : PROP :=
+    ∃ b, ⌜v = ValLiteral (LiteralBool b)⌝.
+  #[global] Instance itype_bool_itype :
+    iType _ itype_bool.
+  Proof.
+    split. apply _.
+  Qed.
+
+  Definition itype_int v : PROP :=
     ∃ i, ⌜v = ValLiteral (LiteralInt i)⌝.
-  #[global] Instance int_type_itype :
-    iType _ int_type.
+  #[global] Instance itype_int_itype :
+    iType _ itype_int.
   Proof.
     split. apply _.
   Qed.
 
-  Definition refined_int_type ϕ v : PROP :=
+  Definition itype_refined_int ϕ v : PROP :=
     ∃ i, ⌜v = ValLiteral (LiteralInt i) ∧ ϕ i⌝.
-  #[global] Instance refined_int_type_itype ϕ :
-    iType _ (refined_int_type ϕ).
+  #[global] Instance itype_refined_int_itype ϕ :
+    iType _ (itype_refined_int ϕ).
   Proof.
     split. apply _.
   Qed.
 
-  Definition int_range_type lb ub :=
-    refined_int_type (λ i, (lb ≤ i < ub)%Z).
+  Definition itype_int_range lb ub :=
+    itype_refined_int (λ i, (lb ≤ i < ub)%Z).
 
-  Definition nat_type v : PROP :=
+  Definition itype_nat v : PROP :=
     ∃ i, ⌜v = ValLiteral (LiteralInt (Z.of_nat i))⌝.
-  #[global] Instance nat_type_itype :
-    iType _ nat_type.
+  #[global] Instance itype_nat_itype :
+    iType _ itype_nat.
   Proof.
     split. apply _.
   Qed.
 
-  Definition refined_nat_type ϕ v : PROP :=
+  Definition itype_refined_nat ϕ v : PROP :=
     ∃ i, ⌜v = ValLiteral (LiteralInt (Z.of_nat i)) ∧ ϕ i⌝.
-  #[global] Instance refined_nat_type_itype ϕ :
-    iType _ (refined_nat_type ϕ).
+  #[global] Instance itype_refined_nat_itype ϕ :
+    iType _ (itype_refined_nat ϕ).
   Proof.
     split. apply _.
   Qed.
 
-  Definition nat_range_type lb ub :=
-    refined_nat_type (λ i, lb ≤ i < ub).
-  Definition nat_upto_type ub :=
-    refined_nat_type (λ i, i < ub).
-End basic_types.
+  Definition itype_nat_range lb ub :=
+    itype_refined_nat (λ i, lb ≤ i < ub).
+  Definition itype_nat_upto ub :=
+    itype_refined_nat (λ i, i < ub).
+End basic.
 
-Section other_types.
+Section other.
   Context `{zebre_G : !ZebreG Σ}.
 
   Implicit Types v fn : val.
 
-  Definition function_type τ1 `{!iType _ τ1} τ2 `{!iType _ τ2} fn : iProp Σ :=
+  Definition itype_fun τ1 `{!iType _ τ1} τ2 `{!iType _ τ2} fn : iProp Σ :=
     □ (∀ v, τ1 v -∗ WP App (Val fn) (Val v) {{ τ2 }}).
-  #[global] Instance function_type_itype τ1 `{!iType _ τ1} τ2 `{!iType _ τ2} :
-    iType _ (function_type τ1 τ2).
+  #[global] Instance itype_fun_itype τ1 `{!iType _ τ1} τ2 `{!iType _ τ2} :
+    iType _ (itype_fun τ1 τ2).
   Proof.
     split. apply _.
   Qed.
 
-  Definition later_type τ `{!iType _ τ} v : iProp Σ :=
+  Definition itype_later τ `{!iType _ τ} v : iProp Σ :=
     ▷ τ v.
-  #[global] Instance later_type_itype τ `{!iType _ τ} :
-    iType _ (later_type τ).
+  #[global] Instance itype_later_itype τ `{!iType _ τ} :
+    iType _ (itype_later τ).
   Proof.
     split. apply _.
   Qed.
-End other_types.
+End other.
 
-Declare Scope itype_scope.
-Delimit Scope itype_scope with T.
+Declare Scope zebre_itype.
+Delimit Scope zebre_itype with T.
 
 Infix "-->" := (
-  function_type
-) : itype_scope.
+  itype_fun
+) : zebre_itype.
 Notation "▷ τ" := (
-  later_type τ
-) : itype_scope.
+  itype_later τ
+) : zebre_itype.
